Rewrote everything to use pre-/post-conditions.

src/Phasers/Phaser.v
@@ -17,10 +17,63 @@ Import HJ.Vars.Map_TID.
 Definition phaser := Map_TID.t taskview.
 
 (**
+  The following record defines the specification of a phaser operation.
+  An operation is issued by a task of type [tid] and targets a [phaser].
+  The pre condition [can_run] must be satisfied to execute the implementation [run] on
+  a given phaser.
+  *)
+
+Record Op := mk_op {
+  can_run: tid -> phaser -> Prop;
+  run: tid -> phaser -> phaser
+}.
+
+(**
+  Function [make] creates a new phaser and registers task [t] with it.
+  Task [t] becomes registered with the initial taskview [Taskview.make].
+*)
+
+Definition make t := add t Taskview.make (Map_TID.empty taskview).
+
+(**
+  Function [update] targets a phaser [ph] and is used internally to mutate
+  the taskview associated with task [t] using function [f] to mutate.
+  If task [t] is not registered in [ph], then the phaser is left unchanged.
+*)
+
+Definition update (t:tid) (f:taskview -> taskview) (ph:phaser) : phaser :=
+  match find t ph with
+  | Some v => add t (f v) ph
+  | None => ph
+  end.
+
+(** For the signal to take any effect the task must be registered with the phaser. *)
+
+Inductive SignalPre (t:tid) (ph:phaser) : Prop :=
+  signal_pre:
+    Map_TID.In t ph ->
+    SignalPre t ph.
+
+(**
+  Signal just applies [Taskview.signal] to the taskview associated with
+  task [t].
+  *)
+
+Definition signal (t:tid) : phaser -> phaser := update t Taskview.signal.
+
+(**
+  We now pair the pre condition with the implementation. This is later used
+  in the definition of the operational semantics.
+  *)
+
+Definition signal_op := mk_op SignalPre signal.
+
+
+(**
   Predicate [Await] holds when all tasks registered in phaser [ph] 
   that have a signal capability have a signal phase of at least [n].
   By only awaiting tasks with a signal capability, predicate [Await]
-  does *not* wait for any task registered with [WAIT_ONLY] mode, regardless
+  does _not_ wait for any task registered with [WAIT_ONLY] mode, regardless
   of its signal phase. Intuitively, this predicate lets a task to wait for
   all members of a phaser to reach a given phase.
   *)
@@ -59,42 +112,43 @@ Inductive Sync : phaser -> tid -> Prop :=
     Sync ph t.
 
 (**
-  Function [make] creates a new phaser and registers task [t] with it.
-  Task [t] becomes registered with the initial taskview [Taskview.make].
-*)
-
-Definition make t := add t Taskview.make (Map_TID.empty taskview).
-
-(**
-  Function [update] targets a phaser [ph] and is used internal to mutate
-  the taskview associated with the given task [t] with function [f].
-  If task [t] is not registered in [ph], then the phaser is left unchanged.
-*)
-
-Definition update (t:tid) (f:taskview -> taskview) (ph:phaser) : phaser :=
-  match find t ph with
-  | Some v => add t (f v) ph
-  | None => ph
-  end.
-
-(**
-  Signal and wait use [update] to apply either [Taskview.signal] or
-  [Taskview.wait] to the registered taskview.
+  Operation wait has two pre-conditions: (i) the issuer must have signalled previously,
+  and (ii) the issuer must synchronize by means of the given phaser with [Sync t ph].
   *)
 
-Definition signal (t:tid) : phaser -> phaser := update t Taskview.signal.
+Inductive WaitPre t ph : Prop  := 
+  wait_pre:
+    forall v,
+    Map_TID.MapsTo t v ph ->
+    Taskview.WaitPre v ->
+    Sync ph t ->
+    WaitPre t ph.
+
+(** Wait then applies wait on the taskview associated with task [t].*)
 
 Definition wait (t:tid) : phaser -> phaser := update t Taskview.wait.
 
-(** Function [drop] removes the taskview associated with the given task. *)
+Definition wait_op := mk_op WaitPre wait.
+
+
+(**
+  Function [drop] removes the taskview associated with the given task.
+  The pre-condition to issue a [drop] is that task [t] must be registered
+  in phaser [ph].
+  *)
+
+Inductive DropPre t (ph:phaser) : Prop :=
+  drop_pre:
+    Map_TID.In t ph ->
+    DropPre t ph.
 
 Definition drop : tid -> phaser -> phaser := @remove taskview.
 
+Definition drop_op := mk_op DropPre drop.
+
 (**
-  Function [register] embodies invoking an [async phased].
-  Operationally, this operation puts a new taskview in the phaser, associated to
-  task [get_task r].
-  The new taskview is a copy of the issuer's taskview, whose mode is set to [get_mode r].
+  Function [register] embodies the invocation of an async phased, and
+  it requires the task being registered and the registration mode of the task.
   *)
 
 Record registry := mk_registry {
@@ -102,91 +156,87 @@ Record registry := mk_registry {
   get_mode: regmode
 }.
 
+(**
+  Register has two pre-conditions: (i) task [get_task r] must be
+  unknown to phaser [ph], and (ii) the mode in registry [r] cannot escalate the
+  capabilities of the issuer.
+*)
+
+Import Regmode.Notations.
+Open Scope reg_scope.
+
+Inductive RegisterPre r t ph : Prop :=
+  register_pre:
+    forall v,
+    ~ Map_TID.In (get_task r) ph ->
+    Map_TID.MapsTo t v ph ->
+    get_mode r <= mode v ->
+    RegisterPre r t ph.
+
+(**
+  Operationally, register adds task [get_task r]  to the phaser, assigning new taskview
+  that is a copy of the issuer's taskview with the mode set to [get_mode r].
+  *)
+
 Definition register (r:registry) (t:tid) (ph:phaser) : phaser := 
   match find t ph with
   | Some v => add (get_task r) (set_mode v (get_mode r)) ph
   | None => ph
   end.
 
-(* begin hide *)
+Definition register_op r := mk_op (RegisterPre r) (register r).
 
 End Defs.
 
-Module Semantics.
 
-  Import Taskview.Semantics.
-  Import Regmode.Notations.
-  Open Scope reg_scope.
-(* end hide *)
+(** The operational semantics define a set of four possible operations:
+  signal, wait, drop (that deregisters the issuer),
+  and register (that adds a new task to the phaser). *)
 
-(** * Small-step Operational Semantics *)
+Inductive op := SIGNAL | WAIT | DROP | REGISTER : registry -> op.
 
-  (** The operational semantics define a set of four possible operations:
-    signal, wait, drop (that deregisters the issuer),
-    and register (that adds a new task to the phaser). *)
+(** Function [eval] interprets operation [o] as its operation specification [Op]. *)
 
-  Inductive op := SIGNAL | WAIT | DROP | REGISTER : registry -> op.
-
-  (** Function [eval] interprets operation [o] as its respective function. *)
-
-  Definition eval o :=
-  match o with
-  | SIGNAL => signal
-  | WAIT => wait
-  | DROP => drop
-  | REGISTER r => register r
-  end.
-
-  (**
-    Relation [Reduces] defines the operational semantics. Two operations are worth detailing.
-    Operation [WAIT] has two pre-conditions: (i) the issuer must have signalled previously,
-    and (ii) the issuer must synchronize by means of the given phaser with [Sync t ph].
-    Operation [REGISTER r] has two pre-conditions: (i) task [get_task r] must be unknown to the phaser,
-    and (ii) the mode in the registry can only pass capabilities that the issuer already has.
-  *)
-
-  Inductive Reduces (ph:phaser) (t:tid) : op -> phaser -> Prop :=
-  | reduces_signal:
-    Map_TID.In t ph ->
-    Reduces ph t SIGNAL (signal t ph)
-  | reduces_wait:
-    forall v,
-    Map_TID.MapsTo t v ph ->
-    wait_phase v < signal_phase v ->
-    Sync ph t ->
-    Reduces ph t WAIT (wait t ph)
-  | reduces_drop:
-    Map_TID.In t ph ->
-    Reduces ph t DROP (drop t ph)
-  | reduces_register:
-    forall v r,
-    ~ Map_TID.In (get_task r) ph ->
-    Map_TID.MapsTo t v ph ->
-    get_mode r <= mode v ->
-    Reduces ph t (REGISTER r) (register r t ph).
-
-  (** Relation [SReducess] simply omits the task and operation of relation [Reduces]. *)
-
-  Inductive SReduces (ph1:phaser) (ph2:phaser) : Prop :=
-    s_reduces:
-      forall t o,
-      Reduces ph1 t o ph2 ->
-      SReduces ph1 ph2.
-
-  (** Finally, we declare a function that converts a [Phaser.op] to a [Taskview.op]. *)
-
-  Definition as_tv_op (o:op) :=
-  match o with
-  | SIGNAL => Some Taskview.Semantics.SIGNAL
-  | WAIT =>  Some Taskview.Semantics.WAIT
-  | _ => None
-  end.
+Definition get_impl o :=
+match o with
+| SIGNAL => signal_op
+| WAIT => wait_op
+| DROP => drop_op
+| REGISTER r => register_op r
+end.
   
+(**
+  Relation [Reduces] defines the operational semantics. Two operations are worth detailing.
+*)
+
+Inductive Reduces ph t o : phaser -> Prop :=
+  reduces:
+    can_run (get_impl o) t ph ->
+    Reduces ph t o (run (get_impl o) t ph).
+
+(** Relation [SReducess] simply omits the task and operation of relation [Reduces]. *)
+
+Inductive SReduces (ph1:phaser) (ph2:phaser) : Prop :=
+  s_reduces:
+    forall t o,
+    Reduces ph1 t o ph2 ->
+    SReduces ph1 ph2.
+
+(** Finally, we declare a function that converts a [Phaser.op] to a [Taskview.op]. *)
+
+Definition as_tv_op (o:op) :=
+match o with
+| SIGNAL => Some Taskview.SIGNAL
+| WAIT =>  Some Taskview.WAIT
+| _ => None
+end.
+
   (* begin hide *)
+Section Facts.
 
   Lemma as_tv_op_inv_signal:
     forall o,
-    as_tv_op o = Some Taskview.Semantics.SIGNAL ->
+    as_tv_op o = Some Taskview.SIGNAL ->
     o = SIGNAL.
   Proof.
     intros.
@@ -195,7 +245,7 @@ Module Semantics.
 
   Lemma as_tv_op_inv_wait:
     forall o,
-    as_tv_op o = Some Taskview.Semantics.WAIT ->
+    as_tv_op o = Some Taskview.WAIT ->
     o = WAIT.
   Proof.
     intros.
@@ -205,7 +255,7 @@ Module Semantics.
   Lemma ph_reduces_spec:
     forall ph t o ph',
     Reduces ph t o ph' ->
-    ph' = eval o t ph.
+    ph' = run (get_impl o) t ph.
   Proof.
     intros.
     destruct o;
@@ -242,6 +292,7 @@ Module Semantics.
     intros.
     inversion H0.
     subst.
+    simpl in *.
     unfold signal.
     auto using ph_update_spec.
   Qed.
@@ -254,7 +305,7 @@ Module Semantics.
   Proof.
     intros.
     inversion H0.
-    subst.
+    subst; simpl in *.
     unfold wait.
     auto using ph_update_spec.
   Qed.
@@ -277,23 +328,21 @@ Module Semantics.
     ph' = Map_TID.add (get_task r) (set_mode v (get_mode r)) ph.
   Proof.
     intros.
-    inversion H0; subst.
+    inversion H0; subst; simpl in *.
     unfold register in *.
     remember (Map_TID.find _ _ ).
     symmetry in Heqo.
-    destruct o.
+    destruct o as [v'|].
     - rewrite Map_TID_Facts.find_mapsto_iff in *.
-      assert (v0 = v). {
+      assert (v' = v). {
         rewrite H in *.
-        inversion H3; auto.
-      }
-      assert (t0 = v). {
-        rewrite H in *.
-        inversion Heqo; auto.
+        inversion Heqo.
+        trivial.
       }
       subst.
       trivial.
-    - apply Map_TID_Extra.mapsto_to_in in H3.
+    - inversion H1.
+      apply Map_TID_Extra.mapsto_to_in in H3.
       apply Map_TID_Facts.not_find_in_iff in Heqo.
       contradiction.
   Qed.
@@ -304,7 +353,9 @@ Module Semantics.
     Map_TID.In t ph.
   Proof.
     intros.
-    inversion H; eauto using Map_TID_Extra.mapsto_to_in.
+    inversion H.
+    destruct o;
+    simpl in *; inversion H0; eauto using Map_TID_Extra.mapsto_to_in.
   Qed.
 
   (* end hide *)
@@ -320,7 +371,7 @@ Module Semantics.
     Reduces ph t o ph' ->
     as_tv_op o = Some o' ->
     Map_TID.MapsTo t v ph ->
-    ph' = Map_TID.add t (Taskview.Semantics.eval o' v) ph.
+    ph' = Map_TID.add t (Taskview.eval o' v) ph.
   Proof.
     intros.
     destruct o'; simpl.
@@ -340,20 +391,21 @@ Module Semantics.
     Reduces ph t o ph' ->
     as_tv_op o = Some o' ->
     Map_TID.MapsTo t v ph ->
-    Taskview.Semantics.Reduces v o' (Taskview.Semantics.eval o' v).
+    Taskview.Reduces v o' (Taskview.eval o' v).
   Proof.
     intros.
     destruct o'; simpl.
     - apply as_tv_op_inv_signal in H0; subst.
-      apply Semantics.tv_reduces_signal.
+      apply tv_reduces_signal.
     - apply as_tv_op_inv_wait in H0; subst.
       inversion H.
-      subst.
-      apply Semantics.tv_reduces_wait.
+      subst; simpl in *.
+      apply tv_reduces_wait.
+      inversion H0.
       assert (v0 = v) by eauto using Map_TID_Facts.MapsTo_fun.
       subst.
       intuition.
   Qed.
 (* begin hide *)
-End Semantics.
+End Facts.
 (* end hide *)
