src/Phasers/Phasermap.v
@@ -13,9 +13,21 @@ Definition phasermap := Map_PHID.t phaser.
 
 Definition make : phasermap := Map_PHID.empty phaser.
 
+Record Op := mk_op {
+  can_run: tid -> phasermap -> Prop;
+  run: tid -> phasermap -> phasermap
+}.
+
 (** Function [new_phaser] places a new empty phaser in the phasermap. *)
 
+Inductive PhNewPre p (t:tid) (m:phasermap) : Prop :=
+  ph_new_pre:
+    ~ Map_PHID.In p m ->
+    PhNewPre p t m.
+
 Definition ph_new (p:phid) (t:tid) : phasermap -> phasermap := Map_PHID.add p (Phaser.make t).
+
+Definition ph_new_op p := mk_op (PhNewPre p) (ph_new p).
 
 (**
   Similarly, to [Phaser.update] function [update] mutates the phaser associated to [p]
@@ -30,85 +42,56 @@ end.
 
 (** We defined signaling a phaser. *)
 
+Inductive PhSignalPre p t m : Prop :=
+  ph_signal_pre:
+    forall ph,
+    Map_PHID.MapsTo p ph m ->
+    SignalPre t ph ->
+    PhSignalPre p t m.
+
 Definition ph_signal p t := update p (Phaser.signal t).
+
+Definition ph_signal_op p := mk_op (PhSignalPre p) (ph_signal p).
 
 (** And droping a phaser. *)
 
+Inductive PhDropPre p t m : Prop :=
+  ph_drop_pre:
+    forall ph,
+    Map_PHID.MapsTo p ph m ->
+    DropPre t ph ->
+    PhDropPre p t m.
+
 Definition ph_drop p t := update p (Phaser.drop t).
 
+Definition ph_drop_op p := mk_op (PhDropPre p) (ph_drop p).
 
 (** Function [foreach] updates all phasers in the phasermap using function [f]. *)
 
 Definition foreach (f:phaser -> phaser) : phasermap -> phasermap := Map_PHID.mapi (fun _ ph => f ph).
 
-(** Function [drop_all] deregisters task [t] from all phasers in the phasermap. *)
+(** Function [signal_all] lets task [t] perform a [Phaser.signal] on all phasers it is registered with. *)
 
-Definition drop_all (t:tid) := foreach (Phaser.drop t).
+Definition signal_all (t:tid) := foreach (Phaser.signal t).
+
+Definition signal_all_op := mk_op (fun _ _ => True) signal_all.
+
+Inductive WaitAllPre t m : Prop :=
+  wait_all_pre:
+    (forall p ph, Map_PHID.MapsTo p ph m -> Map_TID.In t ph -> WaitPre t ph) ->
+    WaitAllPre t m.
 
 (** Function [wait_all] lets task [t] perform a [Phaser.wait] on all phasers it is registered with. *)
 
 Definition wait_all (t:tid) := foreach (Phaser.wait t).
 
-(** Function [signal_all] lets task [t] perform a [Phaser.signal] on all phasers it is registered with. *)
+Definition wait_all_op := mk_op WaitAllPre wait_all.
 
-Definition signal_all (t:tid) := foreach (Phaser.signal t).
+(** Function [drop_all] deregisters task [t] from all phasers in the phasermap. *)
 
-(**
-  We define async phased in two functions: [async] ranges over each phaser in the list 
-  of phasers and uses [async_1] to registers the spawned
-  task in a single phaser. Task [t] registers task [t'] in phaser [first ps]
-  with mode [snd ps].
- *)
+Definition drop_all (t:tid) := foreach (Phaser.drop t).
 
-Definition phased := (phid * regmode) % type.
-
-Definition async_1 (ps:phased) t' t pm :=
-match Map_PHID.find (fst ps) pm with
-| Some ph =>
-  let ph' := register (mk_registry t' (snd ps)) t ph in
-  Map_PHID.add (fst ps) ph' pm
-| _ => pm
-end.
-
-(** Function [async] applies [async_1] to each element of [l]. *)
-
-Fixpoint async l t' t pm :=
-match l with
-| cons ps l => async_1 ps t' t (async l t' t pm)
-| nil => pm
-end.
-
-Module Semantics.
-  Import Regmode.Notations.
-  Require Import HJ.Phasers.Taskview.
-
-  Open Scope reg_scope.
-
-  (**
-   We are now ready to define the closed set of operations on phasermaps.
-   *)
-
-  Inductive op : Type :=
-  | PH_NEW : phid -> op
-  | PH_SIGNAL : phid -> op
-  | PH_DROP : phid -> op
-  | SIGNAL_ALL
-  | WAIT_ALL
-  | DROP_ALL
-  | ASYNC : list phased -> tid -> op.
-  
-  (** Function [eval] interprets an operation as a function. *)
-
-  Definition eval o :=
-  match o with
-  | PH_NEW p => ph_new p
-  | PH_SIGNAL p => ph_signal p
-  | PH_DROP p => ph_drop p
-  | SIGNAL_ALL => signal_all
-  | WAIT_ALL => wait_all
-  | DROP_ALL => drop_all
-  | ASYNC ps t => async ps t
-  end.
+Definition drop_all_op := mk_op (fun _ _ => True) drop_all.
 
   (** Predicate [In t m] holds when task [t] is registered in a phaser of [m]. *)
 
@@ -120,50 +103,89 @@ Module Semantics.
       In t pm.
 
   (**
-    The behaviour of [Async] is defined inductively, not computationally like the remaining
-    operations.
+    Predicate [Phased m t t' ps] holds when:
+    1. task [t] is registered with phaser [fst ps]
+    2. task [t] can register [t'] according to mode [snd ps]
    *)
 
-  Inductive Phased (m:phasermap) (t:tid): list phased -> Prop :=
-    | phased_step:
-      forall p r l v ph,
-      Phased m t l ->
-      Map_PHID.MapsTo p ph m ->
-      Map_TID.MapsTo t v ph ->
-      r <= (mode v) ->
-      Phased m t ((p,r)::l)
-    | phased_nil:
-      Phased m t nil.
+(**
+  Function [async] applies [async_1] to each element of [l], converting
+  each pair to a [registry] object. *)
 
-  Definition eq_phid (p p':phased) := (fst p) = (fst p').
+Definition phased := (phid * regmode) % type.
 
-  (** Finally, we defined the [Reduce] relation. *)
+Inductive Phased (m:phasermap) (t t':tid) (ps:phased) : Prop := 
+  phased_def:
+    forall ph v,
+    Map_PHID.MapsTo (fst ps) ph m ->
+    Map_TID.MapsTo t v ph ->
+    RegisterPre (mk_registry t' (snd ps)) t ph ->
+    Phased m t t' ps.
 
-  Inductive Reduce (m:phasermap) (t:tid): op -> phasermap -> Prop :=
-    | reduce_ph_new:
-      forall p,
-      ~ Map_PHID.In p m ->
-      Reduce m t (PH_NEW p) (ph_new p t m)
-    | reduce_ph_signal:
-      forall p ph,
-      Map_PHID.MapsTo p ph m ->
-      Reduce m t (PH_SIGNAL p) (ph_signal p t m)
-    | reduce_ph_drop:
-      forall p ph,
-      Map_PHID.MapsTo p ph m ->
-      Reduce m t (PH_DROP p) (ph_drop p t m)
-   | reduce_signal_all:
-      Reduce m t SIGNAL_ALL (signal_all t m)
-   | reduce_wait_all:
-     (forall p ph, Map_PHID.MapsTo p ph m -> Map_TID.In t ph -> Sync ph t) ->
-     Reduce m t WAIT_ALL (wait_all t m)
-   | reduce_drop_all:
-      Reduce m t DROP_ALL (drop_all t m)
-   | reduce_async:
-      forall ps t',
-      Phased m t ps ->
-      NoDupA eq_phid ps ->
-      ~ In t' m -> 
-      Reduce m t (ASYNC ps t') (async ps t' t m).
+Definition eq_phid (p p':phased) := (fst p) = (fst p').
 
-End Semantics.
+Inductive AsyncPre ps t' t m : Prop :=
+  async_pre:
+    Forall (Phased m t t') ps ->
+    NoDupA eq_phid ps ->
+    ~ In t' m -> 
+    AsyncPre ps t' t m.
+
+(**
+  We define async phased in two functions: [async] ranges over each phaser in the list 
+  of phasers and uses [async_1] to registers the spawned
+  task in a single phaser. Task [t] registers task [t'] in phaser [first ps]
+  with mode [snd ps].
+ *)
+
+(** Function [async_1] expects the name of the phaser where
+  to register [r]; task [t] is the issuer; phasermap [pm] is the target. *)
+
+Definition async_1 p r t pm :=
+match Map_PHID.find p pm with
+| Some ph => Map_PHID.add p (register r t ph) pm
+| _ => pm
+end.
+
+Fixpoint async (l:list phased) t' t pm :=
+match l with
+| cons (p, r) l => async_1 p (mk_registry t' r) t (async l t' t pm)
+| nil => pm
+end.
+
+Definition async_op l t := mk_op (AsyncPre l t) (async l t).
+
+(**
+  We are now ready to define the closed set of operations on phasermaps.
+ *)
+
+Inductive op : Type :=
+| PH_NEW : phid -> op
+| PH_SIGNAL : phid -> op
+| PH_DROP : phid -> op
+| SIGNAL_ALL
+| WAIT_ALL
+| DROP_ALL
+| ASYNC : list phased -> tid -> op.
+  
+(** Function [eval] interprets an operation as a function. *)
+
+Definition get_impl o :=
+match o with
+| PH_NEW p => ph_new_op p
+| PH_SIGNAL p => ph_signal_op p
+| PH_DROP p => ph_drop_op p
+| SIGNAL_ALL => signal_all_op
+| WAIT_ALL => wait_all_op
+| DROP_ALL => drop_all_op
+| ASYNC ps t => async_op ps t
+end.
+
+
+(** Finally, we define the [Reduce] relation. *)
+
+Inductive Reduces m t o : phasermap -> Prop :=
+  reduces:
+    can_run (get_impl o) t m ->
+    Reduces m t o (run (get_impl o) t m).
+
